RegexCorrectness/Regex/Captures.lean
@@ -1,0 +1,96 @@
+import Regex.Regex.Captures
+import RegexCorrectness.Regex.Basic
+
+set_option autoImplicit false
+
+namespace Regex.Captures
+
+def Valid (self : Captures) : Prop :=
+  self.regex.IsSearchRegex ∧ self.currentPos.Valid self.haystack
+
+theorem next?_some {self self' : Captures} {captured} (h : self.next? = .some (captured, self'))
+  (v : self.Valid) :
+  self'.Valid ∧
+  ∃ l m r groups,
+    v.1.expr.Captures ⟨l, [], m ++ r⟩ ⟨l, m.reverse, r⟩ groups ∧
+    ∀ i, captured.get i = NFA.materializeRegexGroups groups i := by
+  unfold next? at h
+  split at h
+  next lt =>
+    generalize h' : VM.captureNext self.regex.nfa self.regex.wf (self.regex.maxTag + 1) ⟨self.haystack, self.currentPos⟩ = matched at h
+    match matched with
+    | none => simp at h
+    | some matched =>
+      have : 1 ≤ self.regex.maxTag := v.1.le_maxTag
+      have ⟨l, m, r, groups, c, eqv, eq₁, eq₂⟩ := v.1.captures_of_captureNext h' v.2 (by omega)
+
+      simp at h
+      set captured' := CapturedGroups.mk matched.val
+      have hcaptured (i : Nat) : captured'.get i = NFA.materializeRegexGroups groups i := by
+        have eqsize : matched.val.size = self.regex.maxTag + 1 :=
+          matched.property
+        if h₁ : 2 * i + 1 < self.regex.maxTag + 1 then
+          match eq₁ : matched[2 * i]'(by omega) with
+          | none =>
+            have hgroup := (eqv i).1 (by omega)
+            simp [eq₁] at hgroup
+            have : matched.val[2 * i]? = .some .none :=
+              eq₁ ▸ getElem?_pos matched.val (2 * i) (by omega)
+            simp [CapturedGroups.get, this, hgroup]
+          | some v₁ =>
+            match eq₂ : matched[2 * i + 1] with
+            | none =>
+              have hgroup := (eqv i).2 (by omega)
+              simp [eq₂] at hgroup
+              have : matched.val[2 * i + 1]? = .some .none :=
+                eq₂ ▸ getElem?_pos matched.val (2 * i + 1) (by omega)
+              simp [CapturedGroups.get, this, hgroup]
+            | some v₂ =>
+              have hgroup₁ := (eqv i).1 (by omega)
+              have hgroup₂ := (eqv i).2 (by omega)
+              simp [eq₁, eq₂] at hgroup₁ hgroup₂
+              have ⟨_, hgroup₁⟩ := hgroup₁
+              have ⟨_, hgroup₂⟩ := hgroup₂
+              simp [hgroup₁] at hgroup₂
+
+              have eq₁' : matched.val[2 * i]? = .some v₁ :=
+                eq₁ ▸ getElem?_pos matched.val (2 * i) (by omega)
+              have eq₂' : matched.val[2 * i + 1]? = .some v₂ :=
+                eq₂ ▸ getElem?_pos matched.val (2 * i + 1) (by omega)
+              simp [CapturedGroups.get, eq₁', eq₂', hgroup₁, hgroup₂]
+        else
+          match h₂ : NFA.materializeRegexGroups groups i with
+          | none =>
+            have : matched.val[2 * i + 1]? = .none :=
+              getElem?_neg matched.val (2 * i + 1) (by omega)
+            simp [CapturedGroups.get, this]
+          | some _ =>
+            have : (NFA.materializeRegexGroups groups i).isSome := by simp [h₂]
+            have := NFA.mem_tags_of_materializeRegexGroups_some c this
+            have := v.1.maxTag_eq ▸ NFA.lt_of_mem_tags_compile v.1.nfa_eq.symm this
+            simp at h₁
+            omega
+      have : captured'.get 0 = .some (⟨String.utf8Len l⟩, ⟨String.utf8Len l + String.utf8Len m⟩) := by
+        simp [hcaptured 0]
+        have h₁ := (eqv 0).1 (by omega)
+        have h₂ := (eqv 0).2 (by omega)
+        simp [eq₁] at h₁
+        simp [eq₂] at h₂
+        have ⟨_, eq₁⟩ := h₁
+        have ⟨_, eq₂⟩ := h₂
+        simp [eq₂] at eq₁
+        simp [eq₁, eq₂]
+      simp [this] at h
+      split at h
+      next =>
+        simp at h
+        simp [←h, Valid]
+        -- TODO: requires `self.haystack = l ++ m ++ r` so that the position `⟨l ++ m⟩` is valid
+        exact ⟨⟨v.1, sorry⟩, l, m, r, groups, c, hcaptured⟩
+      next nlt =>
+        simp at h
+        simp [←h, Valid]
+        exact ⟨⟨v.1, String.valid_next v.2 lt⟩, l, m, r, groups, c, hcaptured⟩
+  next => simp at h
+
+end Regex.Captures
